pcuic/theories/PCUICOnFreeVars.v
@@ -1104,12 +1104,12 @@ Qed.
 (** This shows preservation by reduction of closed/noccur_between predicates 
   necessary to prove exchange and strengthening lemmas. *)
 Lemma red1_on_free_vars {cf} {P : nat -> bool} {Σ Γ u v} {wfΣ : wf Σ} :
+  red1 Σ Γ u v ->
   on_free_vars P u ->
   on_ctx_free_vars P Γ ->
-  red1 Σ Γ u v ->
   on_free_vars P v.
 Proof.
-  intros hav hctx h.
+  intros h hav hctx.
   induction h using red1_ind_all in P, hav, hctx |- *.
   all: try solve [
     simpl ; constructor ; eapply IHh ;
@@ -1218,14 +1218,12 @@ Proof.
 Qed.
 
 Lemma red_on_free_vars {cf} {P : nat -> bool} {Σ Γ u v} {wfΣ : wf Σ} :
+  red Σ Γ u v ->
   on_free_vars P u ->
   on_ctx_free_vars P Γ ->
-  red Σ Γ u v ->
   on_free_vars P v.
 Proof.
-  intros on onΓ r.
-  induction r; auto.
-  now eapply red1_on_free_vars; tea.
+  induction 1; eauto using red1_on_free_vars.
 Qed.
 
 (*
